identity transformer

MonadTrans.v
@@ -28,12 +28,12 @@ Module Type MonadTransSpec.
                      {A : Type}, M A -> T M A.
   (**[]*)
 
-  Parameter lift_pure : forall {M : Type -> Type} `{Monad M} {A : Type},
+  Axiom lift_pure : forall {M : Type -> Type} `{Monad M} {A : Type},
       @lift M _ A ∘ (@pure M _ A) =
       @pure (T M) (@Monad_Applicative (T M) (TMonad M)) A.
   (**[]*)
 
-  Parameter lift_bind : forall {M : Type -> Type} `{Monad M}
+  Axiom lift_bind : forall {M : Type -> Type} `{Monad M}
                           {A B : Type} (m : M A) (f : A -> M B),
       lift (bind m f) = @bind (T M) (TMonad M) _ _ (lift m) (lift ∘ f).
   (**[]*)
@@ -48,3 +48,91 @@ Module MonadTransFactory (MS : MonadTransSpec).
       lift_bind := @MS.lift_bind }.
   (**[]*)
 End MonadTransFactory.
+
+(** Identity. *)
+Module IdentityMonadTransSpec <: MonadTransSpec.
+  Definition T : (Type -> Type) -> Type -> Type := fun M => M.
+
+  Section TMonadSpec.
+    Context {M : Type -> Type}.
+
+    Context `{HM : Monad M}.
+
+    Definition fmapt {A B : Type} : (A -> B) -> M A -> M B := fmap.
+
+    Lemma fmap_idt : forall {A : Type},
+        fmapt (fun x : A => x) = (fun x : M A => x).
+    Proof. intros. unfold fmapt. apply fmap_id. Qed.
+
+    Lemma fmap_composet : forall {A B C : Type} (f : A -> B) (g : B -> C),
+        fmapt (g ∘ f) = fmapt g ∘ fmapt f.
+    Proof. intros. unfold fmapt. apply fmap_compose. Qed.
+
+    Definition puret {A : Type} : A -> M A := pure.
+
+    Definition fappt {A B : Type} : M (A -> B) -> M A -> M B := fapp.
+
+    Lemma app_identityt : forall {A : Type} (a : M A),
+        fappt (puret (fun x => x)) a = a.
+    Proof. intros. unfold fappt, puret. apply app_identity. Qed.
+
+    Lemma app_homomorphismt : forall {A B : Type} (f : A -> B) (a : A),
+        fappt (puret f) (puret a) = puret (f a).
+    Proof. intros. unfold fappt, puret. apply app_homomorphism. Qed.
+
+    Lemma app_interchanget : forall {A B : Type} (f : M (A -> B)) (a : A),
+        fappt f (puret a) = fappt (puret (fun h => h a)) f.
+    Proof. intros. unfold fappt, puret. apply app_interchange. Qed.
+
+    Lemma app_compositiont :
+      forall {A B C : Type} (f : M (A -> B)) (h : M (B -> C)) (a : M A),
+        fappt h (fappt f a) =
+        fappt (fappt (fappt (puret (@compose A B C)) h) f) a.
+    Proof. intros. unfold fappt, puret. apply app_composition. Qed.
+
+    Lemma app_fmap_puret : forall {A B : Type} (f : A -> B),
+        fmapt f = fappt (puret f).
+    Proof. intros. unfold fmapt, puret. apply app_fmap_pure. Qed.
+
+    Definition bindt {A B : Type} : M A -> (A -> M B) -> M B := bind.
+
+    Lemma pure_leftt : forall {A B : Type} (a : A) (f : A -> M B),
+        bindt (puret a) f = f a.
+    Proof. unfold bindt, puret. intros. apply pure_left. Qed.
+
+    Lemma pure_rightt : forall {A : Type} (m : M A),
+        bindt m puret = m.
+    Proof. intros. unfold bindt, puret. apply pure_right. Qed.
+
+    Lemma bind_assoct :
+      forall {A B C : Type} (m : M A) (k : A -> M B) (h : B -> M C),
+        bindt m (fun a => bindt (k a) h) = bindt (bindt m k) h.
+    Proof. intros. unfold bindt. apply bind_assoc. Qed.
+  End TMonadSpec.
+
+  Instance TMonad (M : Type -> Type) `{Monad M} : Monad M :=
+    { bind := @bindt M _;
+      pure_left := @pure_left M _;
+      pure_right := @pure_right M _;
+      bind_assoc := @bind_assoct M _}.
+  (**[]*)
+
+  Definition lift {M : Type -> Type} `{Monad M}
+             {A : Type} : M A -> M A := fun m => m.
+  (**[]*)
+
+  Lemma lift_pure : forall {M : Type -> Type} `{Monad M} {A : Type},
+      @lift M _ A ∘ (@pure M _ A) =
+      @pure M (@Monad_Applicative M (TMonad M)) A.
+  Proof. intros. unfold lift. extensionality m. reflexivity. Qed.
+
+  Lemma lift_bind : forall {M : Type -> Type} `{Monad M}
+                      {A B : Type} (m : M A) (f : A -> M B),
+      lift (bind m f) = @bind M (TMonad M) _ _ (lift m) (lift ∘ f).
+  Proof. intros. reflexivity. Qed.
+End IdentityMonadTransSpec.
+
+Module IdentityMonadTransFactory :=
+  MonadTransFactory IdentityMonadTransSpec.
+Instance IdentityMonadTrans : MonadTrans (fun M : Type -> Type => M) :=
+  IdentityMonadTransFactory.MonadTransInstance.
